.lake/build/ir/IVI/SchematismEvidence.c
@@ -1,0 +1,273 @@
+// Lean compiler output
+// Module: IVI.SchematismEvidence
+// Imports: Init
+#include <lean/lean.h>
+#if defined(__clang__)
+#pragma clang diagnostic ignored "-Wunused-parameter"
+#pragma clang diagnostic ignored "-Wunused-label"
+#elif defined(__GNUC__) && !defined(__CLANG__)
+#pragma GCC diagnostic ignored "-Wunused-parameter"
+#pragma GCC diagnostic ignored "-Wunused-label"
+#pragma GCC diagnostic ignored "-Wunused-but-set-variable"
+#endif
+#ifdef __cplusplus
+extern "C" {
+#endif
+LEAN_EXPORT lean_object* l_IVI_reprStepEvidence____x40_IVI_SchematismEvidence___hyg_21____boxed(lean_object*, lean_object*);
+static lean_object* l_IVI_reprStepEvidence___redArg___closed__0____x40_IVI_SchematismEvidence___hyg_21_;
+LEAN_EXPORT lean_object* l_IVI_reprStepEvidence____x40_IVI_SchematismEvidence___hyg_21_(uint8_t, lean_object*);
+LEAN_EXPORT lean_object* l_IVI_reprStepEvidence___redArg____x40_IVI_SchematismEvidence___hyg_21_(uint8_t);
+static lean_object* l_IVI_reprStepEvidence___redArg___closed__10____x40_IVI_SchematismEvidence___hyg_21_;
+static lean_object* l_IVI_reprStepEvidence___redArg___closed__3____x40_IVI_SchematismEvidence___hyg_21_;
+lean_object* lean_nat_to_int(lean_object*);
+static lean_object* l_IVI_reprStepEvidence___redArg___closed__9____x40_IVI_SchematismEvidence___hyg_21_;
+static lean_object* l_IVI_instReprStepEvidence___closed__0;
+static lean_object* l_IVI_reprStepEvidence___redArg___closed__4____x40_IVI_SchematismEvidence___hyg_21_;
+static lean_object* l_IVI_reprStepEvidence___redArg___closed__1____x40_IVI_SchematismEvidence___hyg_21_;
+LEAN_EXPORT lean_object* l_IVI_reprStepEvidence___redArg____x40_IVI_SchematismEvidence___hyg_21____boxed(lean_object*);
+lean_object* l_Bool_repr___redArg(uint8_t);
+static lean_object* l_IVI_reprStepEvidence___redArg___closed__6____x40_IVI_SchematismEvidence___hyg_21_;
+static lean_object* l_IVI_reprStepEvidence___redArg___closed__5____x40_IVI_SchematismEvidence___hyg_21_;
+static lean_object* l_IVI_reprStepEvidence___redArg___closed__8____x40_IVI_SchematismEvidence___hyg_21_;
+static lean_object* l_IVI_reprStepEvidence___redArg___closed__7____x40_IVI_SchematismEvidence___hyg_21_;
+LEAN_EXPORT lean_object* l_IVI_instReprStepEvidence;
+static lean_object* l_IVI_reprStepEvidence___redArg___closed__11____x40_IVI_SchematismEvidence___hyg_21_;
+static lean_object* l_IVI_reprStepEvidence___redArg___closed__2____x40_IVI_SchematismEvidence___hyg_21_;
+static lean_object* _init_l_IVI_reprStepEvidence___redArg___closed__0____x40_IVI_SchematismEvidence___hyg_21_() {
+_start:
+{
+lean_object* x_1; 
+x_1 = lean_mk_string_unchecked("{ ", 2, 2);
+return x_1;
+}
+}
+static lean_object* _init_l_IVI_reprStepEvidence___redArg___closed__1____x40_IVI_SchematismEvidence___hyg_21_() {
+_start:
+{
+lean_object* x_1; 
+x_1 = lean_mk_string_unchecked("usedSchematism", 14, 14);
+return x_1;
+}
+}
+static lean_object* _init_l_IVI_reprStepEvidence___redArg___closed__2____x40_IVI_SchematismEvidence___hyg_21_() {
+_start:
+{
+lean_object* x_1; lean_object* x_2; 
+x_1 = l_IVI_reprStepEvidence___redArg___closed__1____x40_IVI_SchematismEvidence___hyg_21_;
+x_2 = lean_alloc_ctor(3, 1, 0);
+lean_ctor_set(x_2, 0, x_1);
+return x_2;
+}
+}
+static lean_object* _init_l_IVI_reprStepEvidence___redArg___closed__3____x40_IVI_SchematismEvidence___hyg_21_() {
+_start:
+{
+lean_object* x_1; lean_object* x_2; lean_object* x_3; 
+x_1 = l_IVI_reprStepEvidence___redArg___closed__2____x40_IVI_SchematismEvidence___hyg_21_;
+x_2 = lean_box(0);
+x_3 = lean_alloc_ctor(5, 2, 0);
+lean_ctor_set(x_3, 0, x_2);
+lean_ctor_set(x_3, 1, x_1);
+return x_3;
+}
+}
+static lean_object* _init_l_IVI_reprStepEvidence___redArg___closed__4____x40_IVI_SchematismEvidence___hyg_21_() {
+_start:
+{
+lean_object* x_1; 
+x_1 = lean_mk_string_unchecked(" := ", 4, 4);
+return x_1;
+}
+}
+static lean_object* _init_l_IVI_reprStepEvidence___redArg___closed__5____x40_IVI_SchematismEvidence___hyg_21_() {
+_start:
+{
+lean_object* x_1; lean_object* x_2; 
+x_1 = l_IVI_reprStepEvidence___redArg___closed__4____x40_IVI_SchematismEvidence___hyg_21_;
+x_2 = lean_alloc_ctor(3, 1, 0);
+lean_ctor_set(x_2, 0, x_1);
+return x_2;
+}
+}
+static lean_object* _init_l_IVI_reprStepEvidence___redArg___closed__6____x40_IVI_SchematismEvidence___hyg_21_() {
+_start:
+{
+lean_object* x_1; lean_object* x_2; lean_object* x_3; 
+x_1 = l_IVI_reprStepEvidence___redArg___closed__5____x40_IVI_SchematismEvidence___hyg_21_;
+x_2 = l_IVI_reprStepEvidence___redArg___closed__3____x40_IVI_SchematismEvidence___hyg_21_;
+x_3 = lean_alloc_ctor(5, 2, 0);
+lean_ctor_set(x_3, 0, x_2);
+lean_ctor_set(x_3, 1, x_1);
+return x_3;
+}
+}
+static lean_object* _init_l_IVI_reprStepEvidence___redArg___closed__7____x40_IVI_SchematismEvidence___hyg_21_() {
+_start:
+{
+lean_object* x_1; lean_object* x_2; 
+x_1 = lean_unsigned_to_nat(18u);
+x_2 = lean_nat_to_int(x_1);
+return x_2;
+}
+}
+static lean_object* _init_l_IVI_reprStepEvidence___redArg___closed__8____x40_IVI_SchematismEvidence___hyg_21_() {
+_start:
+{
+lean_object* x_1; 
+x_1 = lean_mk_string_unchecked(" }", 2, 2);
+return x_1;
+}
+}
+static lean_object* _init_l_IVI_reprStepEvidence___redArg___closed__9____x40_IVI_SchematismEvidence___hyg_21_() {
+_start:
+{
+lean_object* x_1; lean_object* x_2; 
+x_1 = lean_unsigned_to_nat(2u);
+x_2 = lean_nat_to_int(x_1);
+return x_2;
+}
+}
+static lean_object* _init_l_IVI_reprStepEvidence___redArg___closed__10____x40_IVI_SchematismEvidence___hyg_21_() {
+_start:
+{
+lean_object* x_1; lean_object* x_2; 
+x_1 = l_IVI_reprStepEvidence___redArg___closed__0____x40_IVI_SchematismEvidence___hyg_21_;
+x_2 = lean_alloc_ctor(3, 1, 0);
+lean_ctor_set(x_2, 0, x_1);
+return x_2;
+}
+}
+static lean_object* _init_l_IVI_reprStepEvidence___redArg___closed__11____x40_IVI_SchematismEvidence___hyg_21_() {
+_start:
+{
+lean_object* x_1; lean_object* x_2; 
+x_1 = l_IVI_reprStepEvidence___redArg___closed__8____x40_IVI_SchematismEvidence___hyg_21_;
+x_2 = lean_alloc_ctor(3, 1, 0);
+lean_ctor_set(x_2, 0, x_1);
+return x_2;
+}
+}
+LEAN_EXPORT lean_object* l_IVI_reprStepEvidence___redArg____x40_IVI_SchematismEvidence___hyg_21_(uint8_t x_1) {
+_start:
+{
+lean_object* x_2; lean_object* x_3; lean_object* x_4; lean_object* x_5; lean_object* x_6; lean_object* x_7; uint8_t x_8; lean_object* x_9; lean_object* x_10; lean_object* x_11; lean_object* x_12; lean_object* x_13; lean_object* x_14; lean_object* x_15; lean_object* x_16; uint8_t x_17; 
+x_2 = l_IVI_reprStepEvidence___redArg___closed__6____x40_IVI_SchematismEvidence___hyg_21_;
+x_3 = l_IVI_reprStepEvidence___redArg___closed__7____x40_IVI_SchematismEvidence___hyg_21_;
+x_4 = l_Bool_repr___redArg(x_1);
+x_5 = lean_alloc_ctor(4, 2, 0);
+lean_ctor_set(x_5, 0, x_3);
+lean_ctor_set(x_5, 1, x_4);
+x_6 = lean_box(0);
+x_7 = lean_alloc_ctor(6, 1, 1);
+lean_ctor_set(x_7, 0, x_5);
+x_8 = lean_unbox(x_6);
+lean_ctor_set_uint8(x_7, sizeof(void*)*1, x_8);
+x_9 = lean_alloc_ctor(5, 2, 0);
+lean_ctor_set(x_9, 0, x_2);
+lean_ctor_set(x_9, 1, x_7);
+x_10 = l_IVI_reprStepEvidence___redArg___closed__9____x40_IVI_SchematismEvidence___hyg_21_;
+x_11 = l_IVI_reprStepEvidence___redArg___closed__10____x40_IVI_SchematismEvidence___hyg_21_;
+x_12 = lean_alloc_ctor(5, 2, 0);
+lean_ctor_set(x_12, 0, x_11);
+lean_ctor_set(x_12, 1, x_9);
+x_13 = l_IVI_reprStepEvidence___redArg___closed__11____x40_IVI_SchematismEvidence___hyg_21_;
+x_14 = lean_alloc_ctor(5, 2, 0);
+lean_ctor_set(x_14, 0, x_12);
+lean_ctor_set(x_14, 1, x_13);
+x_15 = lean_alloc_ctor(4, 2, 0);
+lean_ctor_set(x_15, 0, x_10);
+lean_ctor_set(x_15, 1, x_14);
+x_16 = lean_alloc_ctor(6, 1, 1);
+lean_ctor_set(x_16, 0, x_15);
+x_17 = lean_unbox(x_6);
+lean_ctor_set_uint8(x_16, sizeof(void*)*1, x_17);
+return x_16;
+}
+}
+LEAN_EXPORT lean_object* l_IVI_reprStepEvidence____x40_IVI_SchematismEvidence___hyg_21_(uint8_t x_1, lean_object* x_2) {
+_start:
+{
+lean_object* x_3; 
+x_3 = l_IVI_reprStepEvidence___redArg____x40_IVI_SchematismEvidence___hyg_21_(x_1);
+return x_3;
+}
+}
+LEAN_EXPORT lean_object* l_IVI_reprStepEvidence___redArg____x40_IVI_SchematismEvidence___hyg_21____boxed(lean_object* x_1) {
+_start:
+{
+uint8_t x_2; lean_object* x_3; 
+x_2 = lean_unbox(x_1);
+lean_dec(x_1);
+x_3 = l_IVI_reprStepEvidence___redArg____x40_IVI_SchematismEvidence___hyg_21_(x_2);
+return x_3;
+}
+}
+LEAN_EXPORT lean_object* l_IVI_reprStepEvidence____x40_IVI_SchematismEvidence___hyg_21____boxed(lean_object* x_1, lean_object* x_2) {
+_start:
+{
+uint8_t x_3; lean_object* x_4; 
+x_3 = lean_unbox(x_1);
+lean_dec(x_1);
+x_4 = l_IVI_reprStepEvidence____x40_IVI_SchematismEvidence___hyg_21_(x_3, x_2);
+lean_dec(x_2);
+return x_4;
+}
+}
+static lean_object* _init_l_IVI_instReprStepEvidence___closed__0() {
+_start:
+{
+lean_object* x_1; 
+x_1 = lean_alloc_closure((void*)(l_IVI_reprStepEvidence____x40_IVI_SchematismEvidence___hyg_21____boxed), 2, 0);
+return x_1;
+}
+}
+static lean_object* _init_l_IVI_instReprStepEvidence() {
+_start:
+{
+lean_object* x_1; 
+x_1 = l_IVI_instReprStepEvidence___closed__0;
+return x_1;
+}
+}
+lean_object* initialize_Init(uint8_t builtin, lean_object*);
+static bool _G_initialized = false;
+LEAN_EXPORT lean_object* initialize_IVI_SchematismEvidence(uint8_t builtin, lean_object* w) {
+lean_object * res;
+if (_G_initialized) return lean_io_result_mk_ok(lean_box(0));
+_G_initialized = true;
+res = initialize_Init(builtin, lean_io_mk_world());
+if (lean_io_result_is_error(res)) return res;
+lean_dec_ref(res);
+l_IVI_reprStepEvidence___redArg___closed__0____x40_IVI_SchematismEvidence___hyg_21_ = _init_l_IVI_reprStepEvidence___redArg___closed__0____x40_IVI_SchematismEvidence___hyg_21_();
+lean_mark_persistent(l_IVI_reprStepEvidence___redArg___closed__0____x40_IVI_SchematismEvidence___hyg_21_);
+l_IVI_reprStepEvidence___redArg___closed__1____x40_IVI_SchematismEvidence___hyg_21_ = _init_l_IVI_reprStepEvidence___redArg___closed__1____x40_IVI_SchematismEvidence___hyg_21_();
+lean_mark_persistent(l_IVI_reprStepEvidence___redArg___closed__1____x40_IVI_SchematismEvidence___hyg_21_);
+l_IVI_reprStepEvidence___redArg___closed__2____x40_IVI_SchematismEvidence___hyg_21_ = _init_l_IVI_reprStepEvidence___redArg___closed__2____x40_IVI_SchematismEvidence___hyg_21_();
+lean_mark_persistent(l_IVI_reprStepEvidence___redArg___closed__2____x40_IVI_SchematismEvidence___hyg_21_);
+l_IVI_reprStepEvidence___redArg___closed__3____x40_IVI_SchematismEvidence___hyg_21_ = _init_l_IVI_reprStepEvidence___redArg___closed__3____x40_IVI_SchematismEvidence___hyg_21_();
+lean_mark_persistent(l_IVI_reprStepEvidence___redArg___closed__3____x40_IVI_SchematismEvidence___hyg_21_);
+l_IVI_reprStepEvidence___redArg___closed__4____x40_IVI_SchematismEvidence___hyg_21_ = _init_l_IVI_reprStepEvidence___redArg___closed__4____x40_IVI_SchematismEvidence___hyg_21_();
+lean_mark_persistent(l_IVI_reprStepEvidence___redArg___closed__4____x40_IVI_SchematismEvidence___hyg_21_);
+l_IVI_reprStepEvidence___redArg___closed__5____x40_IVI_SchematismEvidence___hyg_21_ = _init_l_IVI_reprStepEvidence___redArg___closed__5____x40_IVI_SchematismEvidence___hyg_21_();
+lean_mark_persistent(l_IVI_reprStepEvidence___redArg___closed__5____x40_IVI_SchematismEvidence___hyg_21_);
+l_IVI_reprStepEvidence___redArg___closed__6____x40_IVI_SchematismEvidence___hyg_21_ = _init_l_IVI_reprStepEvidence___redArg___closed__6____x40_IVI_SchematismEvidence___hyg_21_();
+lean_mark_persistent(l_IVI_reprStepEvidence___redArg___closed__6____x40_IVI_SchematismEvidence___hyg_21_);
+l_IVI_reprStepEvidence___redArg___closed__7____x40_IVI_SchematismEvidence___hyg_21_ = _init_l_IVI_reprStepEvidence___redArg___closed__7____x40_IVI_SchematismEvidence___hyg_21_();
+lean_mark_persistent(l_IVI_reprStepEvidence___redArg___closed__7____x40_IVI_SchematismEvidence___hyg_21_);
+l_IVI_reprStepEvidence___redArg___closed__8____x40_IVI_SchematismEvidence___hyg_21_ = _init_l_IVI_reprStepEvidence___redArg___closed__8____x40_IVI_SchematismEvidence___hyg_21_();
+lean_mark_persistent(l_IVI_reprStepEvidence___redArg___closed__8____x40_IVI_SchematismEvidence___hyg_21_);
+l_IVI_reprStepEvidence___redArg___closed__9____x40_IVI_SchematismEvidence___hyg_21_ = _init_l_IVI_reprStepEvidence___redArg___closed__9____x40_IVI_SchematismEvidence___hyg_21_();
+lean_mark_persistent(l_IVI_reprStepEvidence___redArg___closed__9____x40_IVI_SchematismEvidence___hyg_21_);
+l_IVI_reprStepEvidence___redArg___closed__10____x40_IVI_SchematismEvidence___hyg_21_ = _init_l_IVI_reprStepEvidence___redArg___closed__10____x40_IVI_SchematismEvidence___hyg_21_();
+lean_mark_persistent(l_IVI_reprStepEvidence___redArg___closed__10____x40_IVI_SchematismEvidence___hyg_21_);
+l_IVI_reprStepEvidence___redArg___closed__11____x40_IVI_SchematismEvidence___hyg_21_ = _init_l_IVI_reprStepEvidence___redArg___closed__11____x40_IVI_SchematismEvidence___hyg_21_();
+lean_mark_persistent(l_IVI_reprStepEvidence___redArg___closed__11____x40_IVI_SchematismEvidence___hyg_21_);
+l_IVI_instReprStepEvidence___closed__0 = _init_l_IVI_instReprStepEvidence___closed__0();
+lean_mark_persistent(l_IVI_instReprStepEvidence___closed__0);
+l_IVI_instReprStepEvidence = _init_l_IVI_instReprStepEvidence();
+lean_mark_persistent(l_IVI_instReprStepEvidence);
+return lean_io_result_mk_ok(lean_box(0));
+}
+#ifdef __cplusplus
+}
+#endif
